added the materials from SF: var/state/aexp/bexp/cmd/HoareLogic

tso.v
@@ -15,10 +15,10 @@ Updated: 04/09/2014
 
 *)
 
+Require Export XLib.
+
 
 (* TODOS
-
-1. Copy the definitions from SF. Think about how much to copy.
 
 Should have write buffer, thread, lock, etc.
 
@@ -29,6 +29,446 @@ Paper: A better x86 memory model: x86-TSO
 *)
 
 
-Require Export Lib.
+(* ---------------- Var ---------------- *)
+Inductive var : Type :=
+| Var : nat -> var.
+
+Hint Constructors var.
+
+Theorem eq_var_dec : forall v1 v2 : var, {v1 = v2} + {v1 <> v2}.
+Proof with auto.
+  intros.
+  destruct v1 as [n1].
+  destruct v2 as [n2].
+  destruct (eq_nat_dec n1 n2).
+  Case "n1 = n2".
+    left...
+  Case "n2 <> n2".
+    right.
+    intros Hf.
+    apply n.
+    inversion Hf...
+Defined.
+
+Hint Resolve eq_var_dec.
+
+Lemma eq_var : forall (T : Type) (x : var) (p q : T), 
+                 (if eq_var_dec x x then p else q) = p. 
+Proof with auto.
+  intros.
+  destruct (eq_var_dec x x); try reflexivity. 
+  apply ex_falso_quodlibet...
+Qed.
+
+Hint Resolve eq_var.
+
+Lemma neq_var : forall (T : Type) (x y : var) (p q : T),
+                  x <> y -> (if eq_var_dec x y then p else q) = q. 
+Proof with auto.
+  intros.
+  destruct (eq_var_dec x y)...
+  Case "x = y".
+    apply H in e.
+    inversion e.
+Qed.
+
+Hint Resolve neq_var.
+
+Definition X : var := Var 0.
+Definition Y : var := Var 1.
+Definition Z : var := Var 2.
+
+Hint Unfold X.
+Hint Unfold Y.
+Hint Unfold Z.
+(* TODO Do I need to Hint Unfold X/Y/Z ?? *)
+(* ---------------- end of Var ---------------- *)
+
+
+(* ---------------- State ---------------- *)
+Definition state := var -> nat.
+
+Definition empty_state : state := fun _ => 0.
+
+Definition update (st : state) (x : var) (n : nat) : state :=
+  fun x' => if eq_var_dec x x' then n else st x'.
+
+Hint Unfold update.
+
+Theorem update_eq :
+  forall n x st, (update st x n) x = n.
+Proof with auto.
+  intros.
+  unfold update...
+Qed.
+
+Hint Resolve update_eq.
+
+Theorem update_neq :
+  forall x2 x1 n st,
+    x2 <> x1 -> (update st x2 n) x1 = (st x1).
+Proof with auto.
+  intros.
+  unfold update...
+Qed.
+
+Hint Resolve update_neq.
+
+(* Due to most recent assignment, previous assignments are shadowed. *)
+Theorem update_shadow :
+  forall n1 n2 x1 x2 (st : state),
+    (update (update st x2 n1) x2 n2) x1 = (update st x2 n2) x1.
+Proof with auto.
+  intros.
+  unfold update...
+  destruct (eq_var_dec x2 x1)...
+Qed.
+
+Hint Resolve update_shadow.
+
+(* Update a variable to its current value won't "actually" change the state *)
+Theorem update_same : forall n1 x1 x2 (st : state),
+                        st x1 = n1 ->
+                        (update st x1 n1) x2 = st x2.
+Proof with auto.
+  intros.
+  unfold update...
+  destruct (eq_var_dec x1 x2);
+    subst...
+Qed.
+
+Hint Resolve update_same.
+
+(* The order of update doesn't matter *)
+Theorem update_permute :
+  forall n1 n2 x1 x2 x3 st,
+    x2 <> x1 -> 
+    (update (update st x2 n1) x1 n2) x3 = (update (update st x1 n2) x2 n1) x3.
+Proof with auto.
+  intros.
+  unfold update...
+  destruct (eq_var_dec x1 x3)...
+  Case "x1 = x3".
+    destruct (eq_var_dec x2 x3); subst...
+    apply ex_falso_quodlibet...
+Qed.
+
+Hint Resolve update_permute.
+(* ---------------- end of State ---------------- *)
+
+
+(* ---------------- Arithmatic Expressions ---------------- *)
+Inductive aexp : Type :=
+| ANum : nat -> aexp
+| APlus : aexp -> aexp -> aexp
+| AMinus : aexp -> aexp -> aexp
+| AMult : aexp -> aexp -> aexp
+| AVar : var -> aexp.
+
+Hint Constructors aexp.
+
+Tactic Notation "aexp_cases" tactic(first) ident(c) :=
+  first;
+  [ Case_aux c "ANum" | Case_aux c "APlus"
+  | Case_aux c "AMinus" | Case_aux c "AMult"
+  | Case_aux c "AVar" ].
+
+Fixpoint aeval (st : state) (a : aexp) : nat :=
+  match a with
+    | ANum n => n
+    | APlus a1 a2 => (aeval st a1) + (aeval st a2)
+    | AMinus a1 a2 => (aeval st a1) - (aeval st a2)
+    | AMult a1 a2 => (aeval st a1) * (aeval st a2)
+    | AVar x => st x
+  end.
+(* ---------------- end of Arithmatic Expressions ---------------- *)
+
+
+(* ---------------- Boolean Expressions ---------------- *)
+Inductive bexp : Type :=
+| BTrue : bexp
+| BFalse : bexp
+| BNot : bexp -> bexp
+| BAnd : bexp -> bexp -> bexp
+| BOr : bexp -> bexp -> bexp
+| BEq : aexp -> aexp -> bexp
+| BLe : aexp -> aexp -> bexp.
+
+Hint Constructors bexp.
+
+Tactic Notation "bexp_cases" tactic(first) ident(c) :=
+  first;
+  [ Case_aux c "BTrue" | Case_aux c "BFalse" | Case_aux c "BNot"
+  | Case_aux c "BAnd" | Case_aux c "BOr" | Case_aux c "BEq"
+  | Case_aux c "BLe" ].
+
+Fixpoint beval (st : state) (b : bexp) : bool :=
+  match b with
+    | BTrue => true
+    | BFalse => false
+    | BNot b' => negb (beval st b')
+    | BAnd b1 b2 => andb (beval st b2) (beval st b2)
+    | BOr b1 b2 => orb (beval st b1) (beval st b2)
+    | BEq a1 a2 => beq_nat (aeval st a1) (aeval st a2)
+    | BLe a1 a2 => ble_nat (aeval st a1) (aeval st a2)
+  end.
+(* ---------------- end of Boolean Expressions ---------------- *)
+
+
+(* ---------------- Commands ---------------- *)
+Inductive cmd : Type :=
+| CSkip : cmd
+| CAss : var -> aexp -> cmd
+| CSeq : cmd -> cmd -> cmd
+| CIf : bexp -> cmd -> cmd -> cmd
+| CWhile : bexp -> cmd -> cmd.
+
+Hint Constructors cmd.
+
+Tactic Notation "cmd_cases" tactic(first) ident(c) :=
+  first;
+  [ Case_aux c "SKIP" | Case_aux c "::=" | Case_aux c ";;"
+  | Case_aux c "IFB" | Case_aux c "WHILE" ].
+
+Notation "'SKIP'" :=
+  CSkip.
+Notation "x '::=' a" :=
+  (CAss x a) (at level 60).
+Notation "c1 ;; c2" :=
+  (CSeq c1 c2) (at level 80, right associativity).
+Notation "'WHILE' b 'DO' c 'END'" :=
+  (CWhile b c) (at level 80, right associativity).
+Notation "'IFB' b 'THEN' c1 'ELSE' c2 'FI'" :=
+  (CIf b c1 c2) (at level 80, right associativity).
+
+Reserved Notation "c1 '/' st '||' st'" (at level 40, st at level 39).
+
+Inductive ceval : cmd -> state -> state -> Prop :=
+  | CE_Skip : forall st,
+                SKIP / st || st
+  | CE_Ass  : forall st a1 n x,
+                aeval st a1 = n ->
+                (x ::= a1) / st || (update st x n)
+  | CE_Seq : forall c1 c2 st st' st'',
+               c1 / st  || st' ->
+               c2 / st' || st'' ->
+               (c1 ;; c2) / st || st''
+  | CE_IfTrue : forall st st' b c1 (c2 : cmd),
+                  beval st b = true ->
+                  c1 / st || st' ->
+                  (IFB b THEN c1 ELSE c2 FI) / st || st'
+  | CE_IfFalse : forall st st' b c1 c2,
+                   beval st b = false ->
+                   c2 / st || st' ->
+                   (IFB b THEN c1 ELSE c2 FI) / st || st'
+  | CE_WhileEnd : forall b st c,
+                    beval st b = false ->
+                    (WHILE b DO c END) / st || st
+  | CE_WhileLoop : forall st st' st'' b c,
+                     beval st b = true ->
+                     c / st || st' ->
+                     (WHILE b DO c END) / st' || st'' ->
+                     (WHILE b DO c END) / st || st''
+
+where "c1 '/' st '||' st'" := (ceval c1 st st').
+
+Hint Constructors ceval.
+
+Tactic Notation "ceval_cases" tactic(first) ident(c) :=
+  first;
+  [ Case_aux c "CE_Skip" | Case_aux c "CE_Ass"
+  | Case_aux c "CE_Seq" | Case_aux c "CE_IfTrue"
+  | Case_aux c "CE_IfFalse" | Case_aux c "CE_WhileEnd"
+  | Case_aux c "CE_WhileLoop" ].
+
+Ltac inv H := inversion H; subst; clear H.
+Ltac rwinv H1 H2 := rewrite H1 in H2; inv H2.
+Ltac find_rwinv :=
+  match goal with
+      H1: ?E = true, H2: ?E = false |- _ => rwinv H1 H2
+  end.
+
+Theorem ceval_deterministic:
+  forall c st st1 st2,
+    c / st || st1  ->
+    c / st || st2 ->
+    st1 = st2.
+Proof with auto.
+  intros c st st1 st2 E1 E2.
+  generalize dependent st2.
+  ceval_cases (induction E1) Case;
+           intros st2 E2; inversion E2; subst; auto;
+           try find_rwinv.
+  Case "CE_Seq".
+    apply IHE1_1 in H1.
+    subst...
+  Case "CE_WhileLoop".
+    SCase "b1 evaluates to true".
+      apply IHE1_1 in H3.
+      subst.
+      apply IHE1_2...
+Qed.
+
+Hint Resolve ceval_deterministic.
+(* ---------------- end of Commands ---------------- *)
+
+
+(* ---------------- Equivalence ---------------- *)
+(* TODO This may not be used later on.
+   And it is likely for different kinds of optimization. *)
+(* ---------------- end of Equivalence ---------------- *)
+
+
+(* ---------------- Hoare Logic ---------------- *)
+Definition Assertion := state -> Prop.
+
+Definition assert_implies (P Q : Assertion) : Prop :=
+  forall st, P st -> Q st.
+
+Hint Unfold assert_implies.
+
+Notation "P ->> Q" :=
+  (assert_implies P Q) (at level 80) : hoare_spec_scope.
+Open Scope hoare_spec_scope.
+
+Notation "P <<->> Q" :=
+  (P ->> Q /\ Q ->> P) (at level 80) : hoare_spec_scope.
+
+
+Definition hoare_triple (P : Assertion) (c : cmd) (Q : Assertion) : Prop :=
+  forall st st', c / st || st'  ->
+                 P st  ->
+                 Q st'.
+
+Hint Unfold hoare_triple.
+
+Notation "{{ P }}  c  {{ Q }}" :=
+  (hoare_triple P c Q) (at level 90, c at next level)
+  : hoare_spec_scope.
+
+
+Theorem hoare_skip : forall P,
+                       {{P}} SKIP {{P}}.
+Proof with eauto.
+  unfold hoare_triple; intros.
+  inversion H; subst...
+Qed.
+
+Hint Resolve hoare_skip.
+
+Definition assn_sub X a P : Assertion :=
+  fun (st : state) =>
+    P (update st X (aeval st a)).
+
+Hint Unfold assn_sub.
+
+Notation "P [ X |-> a ]" := (assn_sub X a P) (at level 10).
+
+Theorem hoare_asgn : forall Q X a,
+                       {{Q [X |-> a]}} (X ::= a) {{Q}}.
+Proof with eauto.
+  unfold hoare_triple.
+  intros.
+  inversion H; subst...
+Qed.
+
+Hint Resolve hoare_asgn.
+
+Theorem hoare_seq : forall P Q R c1 c2,
+                      {{Q}} c2 {{R}} ->
+                      {{P}} c1 {{Q}} ->
+                      {{P}} c1;;c2 {{R}}.
+Proof with eauto.
+  unfold hoare_triple; intros.
+  inversion H1; subst...
+Qed.
+
+Hint Resolve hoare_seq.
+
+Definition bassn b : Assertion :=
+  fun st => (beval st b = true).
+
+Hint Unfold bassn.
+
+Lemma bexp_eval_true :
+  forall b st, beval st b = true -> (bassn b) st.
+Proof. auto. Qed.
+
+Hint Resolve bexp_eval_true.
+
+Lemma bexp_eval_false : forall b st,
+  beval st b = false -> ~ ((bassn b) st).
+Proof.
+  intros.
+  unfold bassn.
+  intros Hf.
+  find_rwinv.
+Qed.
+
+Hint Resolve bexp_eval_false.
+
+Theorem hoare_if :
+  forall P Q b c1 c2,
+    {{fun st => P st /\ bassn b st}} c1 {{Q}} ->
+    {{fun st => P st /\ ~(bassn b st)}} c2 {{Q}} ->
+    {{P}} (IFB b THEN c1 ELSE c2 FI) {{Q}}.
+Proof with eauto.
+  unfold hoare_triple; intros.
+  inversion H1; subst...
+Qed.
+
+Hint Resolve hoare_if.
+
+Lemma hoare_while : forall P b c,
+  {{fun st => P st /\ bassn b st}} c {{P}} ->
+  {{P}} WHILE b DO c END {{fun st => P st /\ ~ (bassn b st)}}.
+Proof with eauto.
+  intros P b c Hhoare st st' He HP.
+  (* Like we've seen before, we need to reason by induction 
+     on He, because, in the "keep looping" case, its hypotheses 
+     talk about the whole loop instead of just c *)
+  remember (WHILE b DO c END) as wcom eqn:Heqwcom.
+  ceval_cases (induction He) Case;
+    try (inv Heqwcom)...
+Qed.
+
+Hint Resolve hoare_while.
+
+Theorem hoare_consequence_pre : forall (P P' Q : Assertion) c,
+  {{P'}} c {{Q}} ->
+  P ->> P' ->
+  {{P}} c {{Q}}.
+Proof. eauto. Qed.
+
+Hint Resolve hoare_consequence_pre.
+
+Theorem hoare_consequence_post : forall (P Q Q' : Assertion) c,
+  {{P}} c {{Q'}} ->
+  Q' ->> Q ->
+  {{P}} c {{Q}}.
+Proof. eauto. Qed.
+
+Hint Resolve hoare_consequence_post.
+
+Theorem hoare_consequence : forall (P P' Q Q' : Assertion) c,
+  {{P'}} c {{Q'}} ->
+  P ->> P' ->
+  Q' ->> Q ->
+  {{P}} c {{Q}}.
+Proof. eauto. Qed.
+
+Hint Resolve hoare_consequence.
+
+Definition is_wp P c Q :=
+  {{P}} c {{Q}} /\
+  forall P', {{P'}} c {{Q}} -> (P' ->> P).
+
+Hint Unfold is_wp.
+(* ---------------- end of Hoare Logic ---------------- *)
+
+
+(* ---------------- Smallstep Semantics ---------------- *)
+(* TODO Is this needed? *)
+(* ---------------- end of Smallstep Semantics ---------------- *)
 
 
